fix a small one

theories/Nullable.v
@@ -2,6 +2,8 @@ Require Import Coq.Program.Equality.
 From LambdaST Require Import
   Context
   Prefix
+  Environment
+  FV
   Types.
 From Hammer Require Import Tactics.
 
@@ -21,6 +23,10 @@ Inductive NullableCtx : context -> Prop :=
       NullableCtx G ->
       NullableCtx G' ->
       NullableCtx (CtxComma G G')
+  | NullableCtxSemic : forall G G',
+      NullableCtx G ->
+      NullableCtx G' ->
+      NullableCtx (CtxSemic G G')
   .
 Hint Constructors NullableCtx : core.
 
@@ -32,4 +38,18 @@ Theorem empty_and_maximal_means_nullable : forall p s,
 Proof.
   intros p s He Hm Ht.
   dependent induction Ht; sauto lq: on.
+Qed.
+
+Theorem emptyon_and_maximalon_means_nullable : forall eta g,
+  EmptyOn (fv g) eta ->
+  MaximalOn (fv g) eta ->
+  EnvTyped eta g ->
+  NullableCtx g.
+Proof.
+  intros eta g He Hm Ht.
+  dependent induction Ht.
+  - sfirstorder.
+  - sauto use:empty_and_maximal_means_nullable.
+  - hauto l:on.
+  - hauto l:on.
 Qed.
